{
 "cells": [
  {
   "cell_type": "markdown",
   "metadata": {},
   "source": [
    "* We focus on propositional logic, i.e., §7.1-4.\n",
    "\n",
    "* If necessary, refresh your knowledge about natural deduction (see also §7.8 for this purpose).\n",
    "* Use the rules in §7 to do Exercise 7.1.\n",
    "  \n",
    "  * Assume B:\n",
    "    * Assume A:\n",
    "      * $B$ (true)\n",
    "    * $A \\implies B$ (intro)\n",
    "  * $B \\implies (A \\implies B)$ (intro)  \n",
    "\n",
    "  * $y : B, x : A \\vdash ? : B \\implies ? \\equiv y$\n",
    "  * $y : B \\vdash A \\to B : *$\n",
    "  * $y : B \\vdash ? : A \\to B \\implies ? \\equiv \\lambda x : A . y$\n",
    "  * $\\vdash B \\to A \\to B : *$\n",
    "  * $\\vdash ? : B \\to A \\to B \\implies ? \\equiv \\lambda y : B . \\lambda x : A \\to y$\n",
    "\n",
    "  * Assume $A \\implies \\bot$:\n",
    "    * Assume $A$:\n",
    "      * $\\bot$ ($\\implies$-elim)\n",
    "      * $B$ ($\\bot$-elim)\n",
    "    * $A \\implies B$\n",
    "  * $(A \\implies \\bot) \\implies (A \\implies B)$ \n",
    "  * $\\neg A \\implies (A \\implies B)$ ($\\neg$-intro)\n",
    "\n",
    "  * $x : A \\to \\Pi \\alpha : * . \\alpha, y : A \\vdash x y B : B$\n",
    "  * $x : A \\to \\bot, y : A \\vdash x y B : B$\n",
    "  * $x : A \\to \\bot \\vdash A \\to B : *$\n",
    "  * $x : A \\to \\bot \\vdash \\lambda y : A . x y B : A \\to B$\n",
    "  * $\\vdash (A \\to \\bot) \\to (A \\to B) : *$\n",
    "  * $\\vdash \\lambda x : A \\to \\bot . \\lambda y : A . x y B : (A \\to \\bot) \\to (A \\to B)$\n",
    "  \n",
    "  * Assume $A \\implies (B \\implies \\bot)$:\n",
    "    * Assume $A \\implies B$:\n",
    "      * Assume $A$:\n",
    "        * $B$ ($\\implies$-elim)\n",
    "        * $B \\implies \\bot$ ($\\implies$-elim)\n",
    "        * $\\bot$ (Modus Ponens)\n",
    "      * $A \\implies \\bot$ ($\\implies$-intro)\n",
    "    * $(A \\implies B) \\implies (A \\implies \\bot)$ ($\\implies$-intro)\n",
    "  * $(A \\implies (B \\implies \\bot)) \\implies ((A \\implies B) \\implies (A \\implies \\bot))$ ($\\implies$-intro)\n",
    "  * $(A \\implies \\neg B) \\implies ((A \\implies B) \\implies \\neg A)$ ($\\neg$-intro)\n",
    "\n",
    "  * $x : A \\to B \\to \\bot, y : A \\to B, z : A \\vdash x z (y z) : \\bot$\n",
    "  * $x : A \\to B \\to \\bot, y : A \\to B \\vdash A \\to \\bot : *$\n",
    "  * $x : A \\to B \\to \\bot, y : A \\to B \\vdash \\lambda z : A . x z (y z) : A \\to \\bot$\n",
    "  * $x : A \\to B \\to \\bot \\vdash (A \\to B) \\to (A \\to \\bot) : *$\n",
    "  * $x : A \\to B \\to \\bot \\vdash \\lambda y : A \\to B . \\lambda z : A . x z (y z) : (A \\to B) \\to (A \\to \\bot)$\n",
    "  * $\\vdash (A \\to (B \\to \\bot)) \\to ((A \\to B) \\to (A \\to \\bot)) : *$\n",
    "  * $\\vdash \\lambda x : A \\to B \\to \\bot . \\lambda y : A \\to B . \\lambda z : A . x z (y z) : (A \\to (B \\to \\bot)) \\to ((A \\to B) \\to (A \\to \\bot))$\n",
    "\n",
    "  * $B \\implies (A \\implies B)$ (a)\n",
    "  * $\\neg B \\lor (A \\implies B)$ ($\\implies$-intro)\n",
    "  * $(A \\implies B) \\lor \\neg B$ (Commutativity)\n",
    "  * $\\neg (A \\implies B) \\implies \\neg B$ ($\\lor$-elim)\n",
    "\n",
    "  * $x : (A \\to B) \\to \\bot, y : B \\vdash x (\\lambda z : A . y): \\bot$\n",
    "  * $x : (A \\to B) \\to \\bot \\vdash B \\to \\bot : *$\n",
    "  * $x : (A \\to B) \\to \\bot \\vdash \\lambda y : B . x (\\lambda z : A . y) : B \\to \\bot$\n",
    "  * $\\vdash ((A \\to B) \\to \\bot) \\to (B \\to \\bot) : *$\n",
    "  * $\\vdash \\lambda x : (A \\to B) \\to \\bot . \\lambda y : B . x (\\lambda z : A . y) : ((A \\to B) \\to \\bot) \\to (B \\to \\bot)$\n",
    "  \n",
    "* During chapter §7, note the various roles of upper-case latin letters A and lower-case greek letters a.\n",
    "  * As previously discussed, upper-case latin letters represent the generic types and / or sorts, as well as logical variables, and the lower-case greek letters describe the real types.\n",
    "* The long Remark 7.1.2 may be considered \"funny\", especially w.r.t. the \"Note:\" at its end, due to the contrary roles of introduction and elimination.\n",
    "  * The one rule is a backward rule (intro) and the other is a forward rule (elim). But in fact, they are the different surfaces of the same medaillon.   \n",
    "* I Conjunction. On, p 141: \"Find yourself derivations ... (Exercise 7.4)\". Do this.\n",
    "  * $\\land$-elim-left-sec\n",
    "  \n",
    "  * $A : S, B : S, f : \\Pi C : S . (A \\to B \\to C) \\to C \\vdash f A (\\lambda x : A . \\lambda y : B . x) : A$\n",
    "  * $A : S, B : S \\vdash \\lambda f : \\Pi C : S . (A \\to B \\to C) \\to C . f A (\\lambda x : A . \\lambda y : B . x) : (\\Pi C : S . (A \\to B \\to C) \\to C) \\to A$\n",
    "  * $\\vdash \\lambda A, B : S . \\lambda f : \\Pi C : S . (A \\to B \\to C) \\to C . f A (\\lambda x : A . \\lambda y : B . x) : \\Pi A, B : S . (\\Pi C : S . (A \\to B \\to C) \\to C) \\to A$\n",
    "\n",
    "* II Disjunction. On, p 143: \"Formal derivations ... (Exercise 7.7)\". Do this.\n",
    "  * $\\lor$-intro-left-sec\n",
    "\n",
    "  * $A, B : *, x : A, C : *, f : A \\to C, g : B \\to C \\vdash f x : C$\n",
    "  * $A, B : *, x : A, C : *, f : A \\to C \\vdash \\lambda g : B \\to C . f x : (B \\to C) \\to C$\n",
    "  * $A, B : *, x : A, C : * \\vdash \\lambda f : A \\to C . \\lambda g : B \\to C . f x : (A \\to C) \\to (B \\to C) \\to C$\n",
    "  * $A, B : *, x : A \\vdash \\lambda C : * . \\lambda f : A \\to C . \\lambda g : B \\to C . f x : \\Pi C : * . (A \\to C) \\to (B \\to C) \\to C$\n",
    "  * $A, B : * \\vdash \\lambda x : A . \\lambda C : * . \\lambda f : A \\to C . \\lambda g : B \\to C . f x : A \\to \\Pi C : * . (A \\to C) \\to (B \\to C) \\to C$\n",
    "  * $\\vdash \\lambda A, B : * . \\lambda x : A . \\lambda C : * . \\lambda f : A \\to C . \\lambda g : B \\to C . f x : \\Pi A, B : * . A \\to \\Pi C : * . (A \\to C) \\to (B \\to C) \\to C$\n",
    "  \n",
    "  * $\\forall A, B \\in S : A \\implies \\forall C \\in S : (A \\implies C) \\implies (B \\implies C) \\implies C$\n",
    "  \n",
    "* Remark 7.2.1: Digest the \"higher-order\" and more \"abstract\" expressions well. Check that we really need λω, for them.\n",
    "\n",
    "  * $\\neg \\equiv \\lambda \\alpha : * . (\\alpha \\to \\bot)$\n",
    "  * $\\land \\equiv \\lambda \\alpha, \\beta : * . \\Pi \\gamma : * . (\\alpha \\to \\beta \\to \\gamma) \\to \\gamma$\n",
    "  * $\\lor \\equiv \\lambda \\alpha, \\beta : * . \\Pi \\gamma : * . (\\alpha \\to \\gamma) \\to (\\beta \\to \\gamma) \\to \\gamma$\n",
    "\n",
    "  * Type depends on type, so yes, $\\lambda \\omega$ is a must. \n",
    "\n",
    "* Carefully follow the derivation in §7.3, including Remark 7.3.2 ...\n",
    "* How do you think about the development into classical logic in §7.4?\n",
    "* Is this rather cool or rather scary/cheating for your taste?\n",
    "  * Introducing an axiom like this is scary, yes.\n",
    "* Do Exercise 7.2.\n",
    "  \n",
    "  * $i_{DN} : \\Pi \\beta : * . \\neg \\neg \\beta \\to \\beta, A : *, n : \\neg A \\to A \\vdash \\lambda x : \\neg A . x(n x) : \\neg \\neg A$\n",
    "  * $i_{DN} : \\Pi \\beta : * . \\neg \\neg \\beta \\to \\beta, A : *, n : \\neg A \\to A \\vdash i_{DN} A (\\lambda x : \\neg A . x(n x)) : A$\n",
    "  * $i_{DN} : \\Pi \\beta : * . \\neg \\neg \\beta \\to \\beta, A : * \\vdash \\lambda n : \\neg A \\to A . i_{DN} A (\\lambda x : \\neg A . x(n x)) : (\\neg A \\to A) \\to A$\n",
    "  * $i_{DN} : \\Pi \\beta : * . \\neg \\neg \\beta \\to \\beta \\vdash \\lambda A : * . \\lambda n : \\neg A \\to A . i_{DN} A (\\lambda x : \\neg A . x(n x)) : \\Pi A : * . (\\neg A \\to A) \\to A$\n",
    "* If you feel like, go on reading thorough Sections §7.5-6 on predicate logic, but I tend to keep this for the last session."
   ]
  }
 ],
 "metadata": {
  "language_info": {
   "name": "python"
  }
 },
 "nbformat": 4,
 "nbformat_minor": 2
}
