{
 "cells": [
  {
   "cell_type": "markdown",
   "metadata": {},
   "source": [
    "\n",
    "* Read the Foreword.\n",
    "\n",
    "* In the Preface, read at least \"Aim and scope.\"\n",
    "\n",
    "* While reading, think about the difference between the words \"invent\" and \"discover.\"\n",
    "\n",
    "* Read through §1.1 and §1.2 and try to remember what was discussed in class on 19.10.\n",
    "\n",
    "* Make sure you understand Example 1.2.4 and Remark 1.2.5.\n",
    "\n",
    "> Ex 1.2.4: $\\lambda z . ((\\lambda x . x)(\\lambda y . y)) \\to_\\beta \\lambda z . (\\lambda y . y)$\n",
    "\n",
    "> Rm 1.2.5: Application is not the result of applying M to N, but rather the construction of a new expression MN, which may lead to the actual execution of a function.\n",
    "\n",
    "* Consider the authors' statement on p. 6 regarding the definition of lambda terms via abstract syntax and its equivalence to Definition 1.3.2(2). Provide arguments for or against this statement.\n",
    "* * Instead of overloaded use of \"=\", use $L ::= u | (L L) | \\lambda u . L$\n",
    "\n",
    "* Note the overloaded use of \"=\" in the definition of Λ.\n",
    "\n",
    "* If needed, refresh your knowledge of multisets to understand Definition 1.3.5.\n",
    "* * $x, x$ from stochastic\n",
    "* * $\\{|x, x |\\}$\n",
    "* * \\Lbag x, x \\Rbag\n",
    "* * Instead of $\\cup$, use $\\uplus$ for union of multisets.\n",
    "\n",
    "* * Beware that $\\alpha$-equivalence does not imply that the subterms (or the count of subterms) match as well. Different free terms result in different subterms.\n",
    "\n",
    "* Understand in what sense Lemma 1.3.6(2) deserves to be labeled \"Transitivity.\"\n",
    "\n",
    "Provide an inductive definition (analogous to Definition 1.4.1) for the variables BV(M) that occur bound in term M. This should not include the occurring binding variables.\n",
    "* * $BV(x) = \\{\\}$\n",
    "* * $BV(MN) = BV(M) \\cup BV(N)$\n",
    "* * $BV(\\lambda x . M) = BV(M) \\cup (FV(M) \\cap \\{x\\})$\n",
    "\n",
    "* For Definition 1.5.1, read the explanation of the two requirements on p. 10 carefully.\n",
    "\n",
    "* If needed, refresh your knowledge on equivalences/congruences for Definition 1.5.2.\n",
    "\n",
    "* Evaluate whether Definition 1.6.1 is a proper definition and consider the use of \"≡\" instead of just \"=\".\n",
    "\n",
    "* Discuss whether Remark 1.6.3(3) appears to be cyclic.\n",
    "\n",
    "* Go back to Definition 1.5.1 and try to come up with a proper inductive definition for Mx→y yourself.\n",
    "\n",
    "* * $x^{x \\to y} \\equiv y$\n",
    "* * $z^{x \\to y} \\equiv z$ if $z \\not\\equiv x$\n",
    "* * $(M N)^{x \\to y} \\equiv M^{x \\to y} N^{x \\to y}$\n",
    "* * $(\\lambda x . P)^{x \\to y} \\equiv \\lambda x . P$\n",
    "* * $(\\lambda z . P)^{x \\to y} \\equiv \\lambda z . P^{x \\to y}$ if $z \\not\\equiv x$\n",
    "* * (Implied by others: $(\\lambda y . P)^{x \\to y} \\equiv (\\lambda z . P^{y \\to z})^{x \\to y}$)\n",
    "\n",
    "* Examine Lemma 1.6.5 and see if you can understand its proof, even if it is described as \"not hard, but rather boring.\"\n",
    "\n",
    "> Lm 1.6.5: Let $x \\not\\equiv y$ and assume $x \\notin FV(L)$, then $M[x := N][y := L] \\equiv M[y := L][x := N[y := L]]$\n",
    "\n",
    "* * $M[x := N][y := L]$ would contain free x's if $x \\in FV(L)$ and $y \\in M[x := N]$. \n",
    "* * But this is not the case, since $x \\notin FV(L)$. So, all $x$'s and $y$'s are replaced.\n",
    "* * Now, consider $M[y := L]$: $y$'s are replaced by $L$'s.\n",
    "* * If $y \\in FV(N)$: $M[y := L][x := N]$ would yield new free $y$'s. But those $y$'s had to be replaced by $L$'s.\n",
    "* * So a new statement $N' \\equiv N[y := L]$ updates the $y$'s in $N$ to $L$'s. $M[y := L][x := N']$ would work.\n",
    "* * Then: $M[x := N][y := L] \\equiv M[y := L][x := N[y := L]]$  \n",
    "\n",
    "* Make sure you understand why y ∈ FV(L) is assumed in the context of Lemma 1.6.5 (See the drawings on p. 14).\n",
    "\n",
    "* Note that Lemma 1.7.1(3) does not represent a \"term construction,\" despite the preceding text pretending it does.\n",
    "\n",
    "* * (3) It is not a construction (application) step, it is an outcome (substitution) step.\n",
    "\n",
    "Reflect on the potential effects of dropping some of the compatibility rules in Definition 1.8.1.\n",
    "\n",
    "* * Assume $M \\equiv N$ but there is a $L$ s.t. $ML \\not\\equiv NL$ (or $LM \\not\\equiv LN$).\n",
    "* * $M \\equiv \\lambda x : P$. Then $ML \\to_\\beta P[x := L]$ and $NL \\to_\\beta P[x := L]$. They cannot differ in their $\\beta$-normal form.\n",
    "* * $L \\equiv \\lambda x : P$. Then $LM \\to_\\beta P[x := M]$ and $LN \\to_\\beta P[x := N] \\equiv P[x := M]$ have to be different. But this is not possible.\n",
    "* * $\\lambda z . M \\equiv \\lambda z . N$. This is already proven by the second point."
   ]
  },
  {
   "cell_type": "markdown",
   "metadata": {},
   "source": []
  }
 ],
 "metadata": {
  "language_info": {
   "name": "python"
  }
 },
 "nbformat": 4,
 "nbformat_minor": 2
}
