{
 "cells": [
  {
   "cell_type": "markdown",
   "metadata": {},
   "source": [
    "1. In Definition 3.4.4: Is (dom(P),α) a good notation for concatenation?\n",
    "    * Yes, as in Python, you have to specify which list you are unpacking. But as we are looking it through the perspective of mathematicians, it doesn't matter. \n",
    "    * Alternative: In Haskell, all lists are defined recursively using the concatenation comma operator between the head and the tail.\n",
    "    * $\\text{cons} : \\alpha' \\to \\alpha' \\text{list} \\to \\alpha' \\text{list}$\n",
    "    * $\\text{conc}: \\alpha' \\text{list} \\to \\alpha' \\text{list} \\to \\alpha' \\text{list}$\n",
    "1. Do Exercise 3.1 ...\n",
    "    * $\\alpha : *, \\beta : *, f : \\alpha \\to \\beta, x : \\alpha$\n",
    "\n",
    "    * 3 must be defined after 1 and 2\n",
    "    * 4 must be defined after 1\n",
    "\n",
    "    * 1 2 3 4\n",
    "    * 2 1 3 4\n",
    "    * 1 2 4 3\n",
    "    * 2 1 4 3\n",
    "    * 1 4 2 3\n",
    "\n",
    "    Also: 5 contexts in total\n",
    "\n",
    "1. When reading the text after Definition 3.4.7, recall our discussions on premises versus side conditions.\n",
    "\n",
    "    * Form is just a simple conclusion. It can be used as the basis of an structural induction proof. The side conditions are not premises, they are just side conditions, which have to be satisfied by the problem statement. \n",
    "\n",
    "1. What kind of objects are type1, type2, type3 on p 77?\n",
    "\n",
    "    * type_1: $\\alpha \\to \\alpha$\n",
    "    * type_2: $(\\alpha \\to \\alpha) \\to \\alpha \\to \\alpha$\n",
    "    * type_3: $\\Pi \\alpha : * . (\\alpha \\to \\alpha) \\to \\alpha \\to \\alpha$\n",
    "\n",
    "1. Do Exercise 3.2 ...\n",
    "\n",
    "    (-6), $\\{\\alpha , \\beta, \\gamma : *, f : \\alpha \\to \\beta, g : \\beta \\to \\gamma, x : \\alpha\\}$: $f : \\alpha \\to \\beta$\n",
    "\n",
    "    (-5), $\\{\\alpha , \\beta, \\gamma : *, f : \\alpha \\to \\beta, g : \\beta \\to \\gamma, x : \\alpha\\}$: $x : \\alpha$\n",
    "\n",
    "    (-4), $\\{\\alpha , \\beta, \\gamma : *, f : \\alpha \\to \\beta, g : \\beta \\to \\gamma, x : \\alpha\\}$: $f x : \\beta$ (appl) on (-6) and (-5)\n",
    "\n",
    "    (-3), $\\{\\alpha , \\beta, \\gamma : *, f : \\alpha \\to \\beta, g : \\beta \\to \\gamma, x : \\alpha\\}$: $g : \\beta \\to \\gamma$\n",
    "\n",
    "    (-2), $\\{\\alpha , \\beta, \\gamma : *, f : \\alpha \\to \\beta, g : \\beta \\to \\gamma, x : \\alpha\\}$: $g(f x) : \\gamma$ (appl) on (-4) and (-3)\n",
    "\n",
    "    (-1), $\\{\\alpha , \\beta, \\gamma : *\\}$: $\\lambda f : \\alpha \\to \\beta . \\lambda g : \\beta \\to \\gamma . \\lambda x : \\alpha . g(f x) : (\\alpha \\to \\beta) \\to (\\beta \\to \\gamma) \\to \\alpha \\to \\gamma$ (abst) on (-2)\n",
    "\n",
    "    (0), $\\{\\}$: $\\lambda \\alpha , \\beta, \\gamma : * . \\lambda f : \\alpha \\to \\beta . \\lambda g : \\beta \\to \\gamma . \\lambda x : \\alpha . g(f x) : \\Pi \\alpha, \\beta, \\gamma : * . (\\alpha \\to \\beta) \\to (\\beta \\to \\gamma) \\to \\alpha \\to \\gamma$ (abst) on (-1)\n",
    "\n",
    "1. Do Exercise 3.4 ...\n",
    "\n",
    "    * (-12) $\\text{nat}, \\text{bool} : *, \\alpha, \\beta : *, f : \\alpha \\to \\alpha, g : \\alpha \\to \\beta, x : \\alpha  \\vdash f : \\alpha \\to \\alpha$ \n",
    "\n",
    "    * (-11) $\\text{nat}, \\text{bool} : *, \\alpha, \\beta : *, f : \\alpha \\to \\alpha, g : \\alpha \\to \\beta, x : \\alpha  \\vdash x : \\alpha$\n",
    "\n",
    "    * (-10) $\\text{nat}, \\text{bool} : *, \\alpha, \\beta : *, f : \\alpha \\to \\alpha, g : \\alpha \\to \\beta, x : \\alpha  \\vdash f x : \\alpha$ (appl) on (-12) and (-11)\n",
    "\n",
    "    * (-9) $\\text{nat}, \\text{bool} : *, \\alpha, \\beta : *, f : \\alpha \\to \\alpha, g : \\alpha \\to \\beta, x : \\alpha  \\vdash f : \\alpha \\to \\alpha$\n",
    "\n",
    "    * (-8) $\\text{nat}, \\text{bool} : *, \\alpha, \\beta : *, f : \\alpha \\to \\alpha, g : \\alpha \\to \\beta, x : \\alpha  \\vdash f(f x) : \\alpha$ (appl) on (-10) and (-9)\n",
    "\n",
    "    * (-7) $\\text{nat}, \\text{bool} : *, \\alpha, \\beta : *, f : \\alpha \\to \\alpha, g : \\alpha \\to \\beta, x : \\alpha \\vdash g : \\alpha \\to \\beta$\n",
    "\n",
    "    * (-6) $\\text{nat}, \\text{bool} : *, \\alpha, \\beta : *, f : \\alpha \\to \\alpha, g : \\alpha \\to \\beta, x : \\alpha  \\vdash g(f(f x)) : \\beta$ (appl) on (-8) and (-7)\n",
    "\n",
    "    * (-5) $\\text{nat}, \\text{bool} : *, \\alpha, \\beta : * \\vdash (\\lambda f : \\alpha \\to \\alpha . \\lambda g : \\alpha \\to \\beta . \\lambda x : \\alpha . g(f(f x))) : (\\alpha \\to \\alpha) \\to (\\alpha \\to \\beta) \\to \\alpha \\to \\beta$ (abst) on (-6)\n",
    "\n",
    "    * (-4) $\\text{nat}, \\text{bool} : * \\vdash (\\lambda \\alpha, \\beta : * . \\lambda f : \\alpha \\to \\alpha . \\lambda g : \\alpha \\to \\beta . \\lambda x : \\alpha . g(f(f x))) : \\Pi \\alpha, \\beta : * . (\\alpha \\to \\alpha) \\to (\\alpha \\to \\beta) \\to \\alpha \\to \\beta$ (abst) on (-5)\n",
    "\n",
    "    * (-3) $\\text{nat}, \\text{bool} : * \\vdash \\text{nat} : * $\n",
    "\n",
    "    * (-2) $\\text{nat}, \\text{bool} : * \\vdash (\\lambda \\alpha, \\beta : * . \\lambda f : \\alpha \\to \\alpha . \\lambda g : \\alpha \\to \\beta . \\lambda x : \\alpha . g(f(f x))) \\text{nat} : \\Pi \\beta : * . (\\text{nat} \\to \\text{nat}) \\to (\\text{nat} \\to \\beta) \\to \\text{nat} \\to \\beta$ (appl) on (-4) and (-3)\n",
    "\n",
    "    * (-1) $\\text{nat}, \\text{bool} : * \\vdash \\text{bool} : * $\n",
    "\n",
    "    * (0) $\\text{nat}, \\text{bool} : * \\vdash (\\lambda \\alpha, \\beta : * . \\lambda f : \\alpha \\to \\alpha . \\lambda g : \\alpha \\to \\beta . \\lambda x : \\alpha . g(f(f x))) \\text{nat} \\text{bool} : (\\text{nat} \\to \\text{nat}) \\to (\\text{nat} \\to \\text{bool}) \\to \\text{nat} \\to \\text{bool}$ (appl) on (-2) and (-1)\n",
    "\n",
    "1. Do Exercise 3.5 (c) (d) ...\n",
    "\n",
    "    * $\\bot \\equiv \\Pi \\alpha : * . \\alpha; \\Gamma \\equiv \\beta : *, x : \\bot$\n",
    "\n",
    "    * (-1) $\\alpha \\in * \\vdash \\alpha \\in *$ (var) satisfied!\n",
    "    * (0) $\\vdash x : \\Pi \\alpha : * . \\alpha$ (abst_2) on (-1)\n",
    "\n",
    "    * $\\Gamma \\vdash y : \\beta$\n",
    "\n",
    "    * $x(\\beta \\to \\beta), \\lambda y : \\beta . y, \\lambda y : \\beta . x\\beta$\n",
    "\n",
    "    * $\\lambda f : \\beta \\to \\beta \\to \\beta . f(x \\beta) (x \\beta) : A, x((\\beta \\to \\beta \\to \\beta) \\to \\beta) : A$\n",
    "\n",
    "    * (-6) $\\Gamma, f : \\beta \\to \\beta \\to \\beta \\vdash x : \\Pi \\alpha : * . \\alpha$\n",
    "\n",
    "    * (-5) $\\Gamma, f : \\beta \\to \\beta \\to \\beta \\vdash \\beta : *$\n",
    "\n",
    "    * (-4) $\\Gamma, f : \\beta \\to \\beta \\to \\beta \\vdash f : \\beta \\to \\beta \\to \\beta$\n",
    "\n",
    "    * (-3) $\\Gamma, f : \\beta \\to \\beta \\to \\beta \\vdash x \\beta : \\beta$ (appl_2) on (-6) and (-5)\n",
    "\n",
    "    * (-2) $\\Gamma, f : \\beta \\to \\beta \\to \\beta \\vdash f(x \\beta) : \\beta \\to \\beta$ (appl) on (-4) and (-3)\n",
    "\n",
    "    * (-1) $\\Gamma, f : \\beta \\to \\beta \\to \\beta \\vdash f(x \\beta) (x \\beta) : \\beta$ appl on (-3) and (-2)\n",
    "\n",
    "    * (0) $\\Gamma \\vdash \\lambda f : \\beta \\to \\beta \\to \\beta . f(x \\beta) (x \\beta) : (\\beta \\to \\beta \\to \\beta) \\to \\beta$ (abst) on (-1)\n",
    "\n",
    "\n",
    "    * (-2) $\\Gamma \\vdash (\\beta \\to \\beta \\to \\beta) \\to \\beta : * $\n",
    "\n",
    "    * (-1) $\\Gamma \\vdash x : \\Pi \\alpha : * . \\alpha$\n",
    "\n",
    "    * (0) $\\Gamma \\vdash x ((\\beta \\to \\beta \\to \\beta) \\to \\beta) : (\\beta \\to \\beta \\to \\beta) \\to \\beta$ (appl) on (-2) and (-1)\n",
    "\n",
    "1. Do Exercise 3.7 ...\n",
    "\n",
    "    * $\\Gamma \\equiv \\alpha : *, \\beta : *, x : \\alpha \\to \\bot, f : (\\alpha \\to \\alpha) \\to \\alpha$\n",
    "\n",
    "    * All free variables of $\\alpha$ and $\\beta$ are declared in $\\Gamma$\n",
    "\n",
    "    * If $\\alpha \\to \\alpha$ has inhabitant, then $\\alpha$ has inhabitant\n",
    "    * $\\alpha \\to \\alpha$ always has an inhabitant\n",
    "    * Then $\\alpha$ has an inhabitant\n",
    "\n",
    "    * If $\\alpha$ has inhabitant, then $\\bot$ has inhabitant\n",
    "    * Then $\\bot$ has inhabitant\n",
    "\n",
    "    * If and only if $\\bot \\beta$ has an inhabitant, $\\beta$ has an inhabitant as well.\n",
    "    * Select $\\beta$ as the inhabitant of $\\bot$.\n",
    "    * Select $y : \\bot \\beta$ as the inhabitant of $\\bot \\beta$\n",
    "    * Then $\\beta$ has the same inhabitant.\n",
    "\n",
    "    * Now the real derivation proof\n",
    "\n",
    "    * $a \\equiv f(\\lambda y : \\alpha . y)$\n",
    "    * $x a : \\bot$\n",
    "    * $(x a) \\beta : \\beta$\n",
    "    * $(x (f (\\lambda y : \\alpha . y))) \\beta : \\beta$\n",
    "    * Make derivation proof and get the same results. \n",
    "\n",
    "1. Try Exercise 3.21 ...\n",
    "\n",
    "    * $FTV(A)$\n",
    "\n",
    "    Types Definition\n",
    "    * $FTV(\\alpha) \\triangleq \\{\\alpha\\}$\n",
    "    * $FTV(\\sigma \\to \\tau) \\triangleq FTV(\\sigma) \\cup FTV(\\tau)$\n",
    "    * $FTV(\\Pi \\alpha : * . \\sigma) \\triangleq FTV(\\sigma) \\backslash \\{\\alpha\\}$\n",
    "\n",
    "    Terms Definition\n",
    "    * $FTV(x) \\triangleq \\{\\}$\n",
    "    * $FTV(MN) \\triangleq FTV(M) \\cup FTV(N)$\n",
    "    * $FTV(M \\tau) \\triangleq FTV(M) \\cup FTV(\\tau)$\n",
    "    * $FTV(\\lambda x : \\tau . M) \\triangleq FTV(M) \\cup FTV(\\tau)$\n",
    "    * $FTV(\\lambda \\alpha : * . M) \\triangleq FTV(M) \\backslash \\{\\alpha\\}$\n",
    "\n",
    "1. Definition 3.6.1: Recall our discussions on 1.6.3(3) leading us to explicitly define $M^{x \\to y}$ in Definition 1.5.1.\n",
    "\n",
    "1. Now, the type variable renaming just defines – as in 1.6.3(3) – renaming via substitution. Is this properly defined? Or is it cyclic?\n",
    "1. Try Exercise 3.19 ...\n",
    "1. Lemma 3.6.4: Why is 2.10.10 missing in the list?\n",
    "\n",
    "    * In $\\lambda C$ and its subsystems, the questions of Well-typedness and Type Checking are decidable. The qquetsion of Term Finding, however, is decidable in $\\lambda\\to$ and $\\lambda \\omega$, but undecidable in all other systems. This is understandable if we recall that there is no way to proof or disproof any arbitrary theorem. \n",
    "\n",
    "1. How would you write out the adaptation of 2.10.5(3) according to the following suggestion?\n",
    "\n",
    "    * Permutation Lemma \n",
    "    \n",
    "    * Condensing Lemma $\\Gamma | FV(M) \\vdash M$ extend over type variables as well. \n",
    "\n",
    "1. Carefully read and check the last paragraph on p81 stretching over to p82.\n",
    "1. Do Exercise 3.10 ...\n",
    "\n",
    "    * $M \\equiv \\lambda x : (\\Pi \\alpha : * . \\alpha \\to \\alpha) . x(\\sigma \\to \\sigma) (x \\sigma)$\n",
    "\n",
    "    * (-7) $x : (\\Pi \\alpha : * . \\alpha \\to \\alpha) \\vdash x : (\\Pi \\alpha : * . \\alpha \\to \\alpha)$ \n",
    "\n",
    "    * (-6) $x : (\\Pi \\alpha : * . \\alpha \\to \\alpha) \\vdash \\sigma \\to \\sigma : *$ \n",
    "\n",
    "    * (-5) $x : (\\Pi \\alpha : * . \\alpha \\to \\alpha) \\vdash x : (\\Pi \\alpha : * . \\alpha \\to \\alpha)$\n",
    "\n",
    "    * (-4) $x : (\\Pi \\alpha : * . \\alpha \\to \\alpha) \\vdash \\sigma : *$ \n",
    "\n",
    "    * (-3) $x : (\\Pi \\alpha : * . \\alpha \\to \\alpha) \\vdash x(\\sigma \\to \\sigma) : (\\sigma \\to \\sigma) \\to (\\sigma \\to \\sigma)$ (appl) on (-7) and (-6) \n",
    "\n",
    "    * (-2) $x : (\\Pi \\alpha : * . \\alpha \\to \\alpha) \\vdash x \\sigma : \\sigma \\to \\sigma$ (appl) on (-5) and (-4) \n",
    "\n",
    "    * (-1) $x : (\\Pi \\alpha : * . \\alpha \\to \\alpha) \\vdash x(\\sigma \\to \\sigma) (x \\sigma) : \\sigma \\to \\sigma$ (appl) on (-3) and (-2)\n",
    "\n",
    "    * (0) $\\vdash \\lambda x : (\\Pi \\alpha : * . \\alpha \\to \\alpha) . x(\\sigma \\to \\sigma) (x \\sigma) : (\\Pi \\alpha : * . \\alpha \\to \\alpha) \\to \\sigma \\to \\sigma$ (abst) on (-1)\n",
    "\n",
    "    * Find $N$ s.t. $M N$ is legal, which adds type information to $(\\lambda x . x x)(\\lambda y . y)$\n",
    "\n",
    "    * $N \\equiv \\lambda \\alpha : * . \\lambda y : \\alpha . y$ then $M N : \\sigma \\to \\sigma$, and it should always hold as true."
   ]
  },
  {
   "cell_type": "markdown",
   "metadata": {},
   "source": []
  }
 ],
 "metadata": {
  "language_info": {
   "name": "python"
  }
 },
 "nbformat": 4,
 "nbformat_minor": 2
}
