{
 "cells": [
  {
   "cell_type": "markdown",
   "metadata": {},
   "source": [
    "* Directly compare the rule sets in Figures 4.1 and 5.1. ...\n",
    "\n",
    "    * (form) \n",
    "        * $\\Gamma \\vdash A : s$ and $\\Gamma \\vdash B : s$ implies $\\Gamma \\vdash A \\to B : s$\n",
    "        * $\\Gamma \\vdash A : *$ and $\\Gamma, x : A \\vdash B : s$ implies $\\Gamma \\vdash \\Pi x : A . B : s$\n",
    "    * (appl) \n",
    "        * $\\Gamma \\vdash M : A \\to B$ and $\\Gamma \\vdash N : A$ implies $\\Gamma \\vdash M N : B$\n",
    "        * $\\Gamma \\vdash M : \\Pi x : A . B$ and $\\Gamma \\vdash N : A$ implies $\\Gamma \\vdash M N : B[x := N]$\n",
    "    * (abst) \n",
    "        * $\\Gamma, x : A \\vdash M : B$ and $\\Gamma \\vdash A \\to B : s$ implies $\\Gamma \\vdash \\lambda x : A . M : A \\to B$\n",
    "        * $\\Gamma, x : A \\vdash M : B$ and $\\Gamma \\vdash \\Pi x : A . B : s$ implies $\\Gamma \\vdash \\lambda x : A . M : \\Pi x : A . B$\n",
    "\n",
    "    * $\\Pi$ reappears, since the terms $x$ may appear freely in type $A$.\n",
    "    * $\\lambda x : A . M$ is the only possible function format given $A : *$.\n",
    "\n",
    "* Do you agree that \"upgrade\" and \"downgrade\" are properly chosen words on p 106 in (i) and (ii)?\n",
    "\n",
    "    * I think on the first sight yes. If there is a hierarchy between terms, types, kinds, super-kinds, super-super-kinds etc., we could have said that it goes upwards from terms to types. \n",
    "    * Otherwise, I disagree. This is just another extension of a cube, and they are both apples and oranges. \n",
    "\n",
    "* Notation 5.2.1 is important!\n",
    "* Carefully check the derivation in ยง 5.3.\n",
    "* Refresh your knowledge about functional completeness of (propositional) logic.\n",
    "* In \"IV\" on p 111, I have some doubts about the \"string of equivalences\". What about you?\n",
    "* Try to do Exercise 5.4 for yourself.\n",
    "\n",
    "    * A kind is legal, if we can derive it using $\\{\\}$. Sort rule clearly says that $* : \\square$ holds always true. Same isn't true for $\\square$, since there is no way to derive it. The contradiction relies on the set theory, where it is stated that there can be no super-set of all sets. \n",
    "\n",
    "    * Let $A, B \\in S$\n",
    "        * Assume $A \\implies (A \\implies B)$\n",
    "            * Assume $A$ \n",
    "                * $A \\implies B$ ($\\implies$-elim)\n",
    "                * $B$\n",
    "            * $A \\implies B$ ($\\implies$-intro)\n",
    "        * $(A \\implies (A \\implies B)) \\implies (A \\implies B)$ ($\\implies$-intro)\n",
    "    * $\\forall A, B \\in S . (A \\implies (A \\implies B)) \\implies (A \\implies B)$ ($\\forall$-intro) \n",
    "\n",
    "* Do Exercise 5.5.\n",
    "\n",
    "    * Let $A, B \\in S$\n",
    "        * Assume $A$\n",
    "            * Assume $A \\implies B$\n",
    "                * $B$ ($\\implies$-elim)\n",
    "            * $(A \\implies B) \\implies B$ ($\\implies$-intro)\n",
    "        * $A \\implies (A \\implies B) \\implies B$ ($\\implies$-intro)\n",
    "    * $\\forall A, B \\in S . A \\implies (A \\implies B) \\implies B$ ($\\forall$-intro)\n",
    "\n",
    "* Try to do Example 5.12 ...  \n",
    "\n",
    "    * $\\Gamma \\equiv S : *, R : S \\to S \\to *, u : \\Pi x , y : S . R x y \\to R y x, v : \\Pi x , y, z : S . R x y \\to R x z \\to R y z$\n",
    "\n",
    "    * --- BEGIN GAMMA --- \n",
    "    * Let $S : *$\n",
    "    * Let $R : S \\to S \\to *$\n",
    "    * Let $u : \\Pi x , y : S . R x y \\to R y x$\n",
    "    * Let $v : \\Pi x , y, z : S . R x y \\to R x z \\to R y z$ \n",
    "    * --- END GAMMA --- \n",
    "\n",
    "    * (-23) $x, y : S, p : R x y \\vdash u : \\lambda x, y : S . R x y \\to R y x$ (VAR)\n",
    "    * (-22) $x, y : S, p : R x y \\vdash y : S$ (VAR)\n",
    "    * (-21) $x, y : S, p : R x y \\vdash u y : \\lambda x : S . R x y \\to R y x$ (appl) on (-23) and (-22)\n",
    "    * (-20) $x, y : S, p : R x y \\vdash x : S $ (VAR)\n",
    "    * (-19) $x, y : S, p : R x y \\vdash u y x : R x y \\to R y x$ (appl) on (-21) and (-20)\n",
    "    * (-18) $x, y : S, p : R x y \\vdash p : R x y$ (VAR)\n",
    "    * (-17) $x, y : S, p : R x y, t, s : S \\vdash v : \\Pi x , y, z : S . R x y \\to R x z \\to R y z$ (VAR)\n",
    "    * (-16) $x, y : S, p : R x y, t, s : S \\vdash t : S$ (VAR)\n",
    "    * (-15) $x, y : S, p : R x y, t, s : S \\vdash v t : \\Pi x , y : S . R x y \\to R x t \\to R y t$ (appl) on (-17) and (-16)\n",
    "    * (-14) $x, y : S, p : R x y, t, s : S \\vdash t : S$ (VAR)\n",
    "    * (-13) $x, y : S, p : R x y, t, s : S \\vdash v t t : \\Pi x : S . R x t \\to R x t \\to R t t$ (appl) on (-15) and (-14)\n",
    "    * (-12) $x, y : S, p : R x y, t, s : S \\vdash s : S$ (VAR)\n",
    "    * (-11) $x, y : S, p : R x y, t, s : S \\vdash v t t s : R s t \\to R s t \\to R t t$ (appl) on (-13) and (-12)\n",
    "    * (-10) $x, y : S, p : R x y \\vdash \\lambda t, s : S . v t t s : \\Pi t, s : S : R s t \\to R s t \\to R t t$ (abst) on (-11)\n",
    "    * (-9) $x, y : S,  \\vdash y : S$ (VAR)\n",
    "    * (-8) $x, y : S, p : R x y \\vdash (\\lambda t, s : S . v t t s) y : \\Pi t : S : R y t \\to R y t \\to R t t$ (appl) on (-10) and (-9)\n",
    "    * (-7) $x, y : S, p : R x y \\vdash x : S$ (VAR)\n",
    "    * (-6) $x, y : S, p : R x y \\vdash (\\lambda t, s : S . v t t s) y x : R y x \\to R y x \\to R x x$ (appl) on (-8) and (-7)\n",
    "    * (-5) $x, y : S, p : R x y \\vdash u y x p : R y x$ (appl) on (-19) and (-18)\n",
    "    * (-4) $x, y : S, p : R x y \\vdash (\\lambda t, s : S . v t t s) y x (u y x p) : R y x \\to R x x$ (appl) on (-6) and (-5)\n",
    "    * (-3) $x, y : S, p : R x y \\vdash u y x p : R y x$ (appl) on (-19) and (-18)\n",
    "    * (-2) $x, y : S, p : R x y \\vdash (\\lambda t, s : S . v t t s) y x (u y x p) (u y x p) : R x x$ (appl) on (-4) and (-3)\n",
    "    * (-1) $x, y : S \\vdash \\lambda p : R x y . (\\lambda t, s : S . v t t s) y x (u y x p) (u y x p) : R x y \\to R x x$ (abst) on (-2)\n",
    "    * (0) $\\vdash \\lambda x, y : S . \\lambda p : R x y . (\\lambda t, s : S . v t t s) y x (u y x p) (u y x p) : \\Pi x, y : S . R x y \\to R x x$ (abst) on (-1)\n",
    "\n",
    "    * (-18) $x, y, z : S, p : R x y, q : R y z, r, s, t : S \\vdash v : R x y \\to R x z \\to R y z$ (VAR)\n",
    "    * (-17) $x, y, z : S, p : R x y, q : R y z, r, s, t : S \\vdash r, s, t : S$ (VAR)\n",
    "    * (-16) $x, y, z : S, p : R x y, q : R y z \\vdash u: \\lambda x, y : S . R x y \\to R y x$ (VAR)\n",
    "    * (-15) $x, y, z : S, p : R x y, q : R y z \\vdash y: S$ (VAR)\n",
    "    * (-14) $x, y, z : S, p : R x y, q : R y z, r, s, t : S \\vdash v r s t : R r s \\to R r t \\to R s t$ (appl) on (-18) and (-17)\n",
    "    * (-13) $x, y, z : S, p : R x y, q : R y z \\vdash u y: \\lambda x : S . R x y \\to R y x$ (appl) on (-16) and (-15)\n",
    "    * (-12) $x, y, z : S, p : R x y, q : R y z \\vdash x: S$ (VAR)\n",
    "    * (-11) $x, y, z : S, p : R x y, q : R y z \\vdash \\lambda r, s, t : S . v r s t: R r s \\to R r t \\to R s t$ (abst) on (-14)\n",
    "    * (-10) $x, y, z : S, p : R x y, q : R y z \\vdash x, y, z: S$ (VAR)\n",
    "    * (-9) $x, y, z : S, p : R x y, q : R y z \\vdash u y x: R x y \\to R y x$ (appl) on (-13) and (-12)\n",
    "    * (-8) $x, y, z : S, p : R x y, q : R y z \\vdash p: R x y$ (VAR)\n",
    "    * (-7) $x, y, z : S, p : R x y, q : R y z \\vdash (\\lambda r, s, t : S . v r s t) y x z: R y x \\to R y z \\to R x z$ (appl) on (-11) and (-10)\n",
    "    * (-6) $x, y, z : S, p : R x y, q : R y z \\vdash u y x p: R y x$ (appl) on (-9) and (-8)\n",
    "    * (-5) $x, y, z : S, p : R x y, q : R y z \\vdash ((\\lambda r, s, t : S . v r s t) y x z) (u y x p): R y z \\to R x z$ (appl) on (-7) and (-6)\n",
    "    * (-4) $x, y, z : S, p : R x y, q : R y z \\vdash q: R y z$ (VAR)\n",
    "    * (-3) $x, y, z : S, p : R x y, q : R y z \\vdash ((\\lambda r, s, t : S . v r s t) y x z) (u y x p) q: R x z$ (appl) on (-5) and (-4)\n",
    "    * (-2) $x, y, z : S, p : R x y \\vdash \\lambda q : R y z . ((\\lambda r, s, t : S . v r s t) y x z) (u y x p) q : R y z \\to R x z$ (abst) on (-3)\n",
    "    * (-1) $x, y, z : S \\vdash \\lambda p : R x y . (\\lambda q : R y z . ((\\lambda r, s, t : S . v r s t) y x z) (u y x p) q) : R x y \\to R y z \\to R x z$ (abst) on (-2)\n",
    "    * (0) $\\vdash \\lambda x, y, z : S . (\\lambda p : R x y . (\\lambda q : R y z . ((\\lambda r, s, t : S . v r s t) y x z) (u y x p) q)) : \\Pi x, y, z : S . R x y \\to R y z \\to R x z$ (abst) on (-1)\n",
    "\n",
    "* Watch \"Propositions as types\" by Phil Wadler (a bit over 40 minutes in total). It is worth it."
   ]
  }
 ],
 "metadata": {
  "language_info": {
   "name": "python"
  }
 },
 "nbformat": 4,
 "nbformat_minor": 2
}
